\documentclass[letterpaper, 11pt]{article}

% Standard packages
\usepackage{amsmath, amsthm, latexsym, amssymb, graphicx, color, mathtools, geometry}

% Simplifies margin settings
\usepackage{geometry}
\geometry{margin=1in,headsep=.25in}

% Puts list item indicators in bold; makes flush with previous margin
\renewcommand\labelenumi{\bf\theenumi.}
\renewcommand\labelenumii{\bf\theenumii.}
\setlength\leftmargini{1.4em}
\setlength\leftmarginii{1.4em}

% Flexibility for headers and footers
\usepackage{fancyhdr}
\usepackage{datetime2}


\pagestyle{fancyplain}
\fancyhf{} %clear all header and footer fields
\cfoot{\bf \small Page \thepage}
\headsep 0.2in
\thispagestyle{empty}

\usepackage[pdftex]{hyperref}
\hypersetup{
    unicode=false,          % non-Latin characters in Acrobat's bookmarks
    pdftoolbar=true,        % show Acrobat's toolbar?
    pdfmenubar=true,        % show Acrobat's menu?
    pdffitwindow=true,      % page fit to window when opened
    pdftitle={My title},    % title
    pdfauthor={Author},     % author
    pdfsubject={Subject},   % subject of the document
    pdfnewwindow=true,      % links in new window
    pdfkeywords={keywords}, % list of keywords
    colorlinks=true,        % false: boxed links; true: colored links
    linkcolor=black,        % color of internal links
    citecolor=green,        % color of links to bibliography
    filecolor=magenta,      % color of file links
    urlcolor=blue           % color of external links
}

\renewcommand{\headrulewidth}{0pt}

\parindent 0in
\parskip 12pt

\begin{document}

\title{Homework Template}

\begin{center}
    {
        \large
        \bf
        CS-E4850 Computer Vision\\
        Exercise Round \#6\\
        Submitted by Chen\ Xu, ID 000000\\
        \today
    }
\end{center}

\bigskip

\textbf{Exercise 1. Least-squares fitting for affine transformations.}\\
a)
\textbf{Solution}\\
\begin{align*}
    E & =\sum_{i=1}^{n}
    \begin{Vmatrix}
        \textbf{x}'_i-\textbf{M}\textbf{x}_i-\textbf{t} \\
    \end{Vmatrix}^2                                 \\
      & =\sum_{i=1}^{n}
    \begin{Vmatrix}
        \begin{bmatrix}
            x'_i \\
            y'_i \\
        \end{bmatrix}
        -
        \begin{bmatrix}
            m_1 & m_2 \\
            m_3 & m_4 \\
        \end{bmatrix}
        \begin{bmatrix}
            x_i \\
            y_i \\
        \end{bmatrix}
        -
        \begin{bmatrix}
            t_1 \\
            t_2 \\
        \end{bmatrix}
    \end{Vmatrix}^2                                                        \\
      & =\sum_{i=1}^{n}
    \begin{Vmatrix}
        \begin{bmatrix}
            x'_i-m_1 x_i-m_2 y_i-t_1 \\
            y'_i-m_3 x_i-m_4 y_i-t_2 \\
        \end{bmatrix}
    \end{Vmatrix}^2                                                        \\
      & =\sum_{i=1}^{n} ((m_1 x_i+m_2 y_i+t_1-x'_i)^2+(m_3 x_i+m_4 y_i+t_2-y'_i)^2)
\end{align*}

\begin{align*}
    \frac{\partial E}{\partial m_1} & =\frac{\partial}{\partial m_1}\sum_{i=1}^{n} ((m_1 x_i+m_2 y_i+t_1-x'_i)^2+(m_3 x_i+m_4 y_i+t_2-y'_i)^2) \\
                                    & =2\sum_{i=1}^{n}x_i(m_1 x_i+m_2 y_i+t_1-x'_i)                                                            \\
    \frac{\partial E}{\partial m_2} & =2\sum_{i=1}^{n}y_i(m_1 x_i+m_2 y_i+t_1-x'_i)                                                            \\
    \frac{\partial E}{\partial m_3} & =2\sum_{i=1}^{n}x_i(m_3 x_i+m_4 y_i+t_2-y'_i)                                                            \\
    \frac{\partial E}{\partial m_4} & =2\sum_{i=1}^{n}y_i(m_3 x_i+m_4 y_i+t_2-y'_i)                                                            \\
    \frac{\partial E}{\partial t_1} & =2\sum_{i=1}^{n}(m_1 x_i+m_2 y_i+t_1-x'_i)                                                               \\
    \frac{\partial E}{\partial t_2} & =2\sum_{i=1}^{n}(m_3 x_i+m_4 y_i+t_2-y'_i)                                                               \\
\end{align*}
\newpage
b)
\begin{proof}
    By setting above gradients to zero, one can get:\\
    \begin{align*}
        \begin{bmatrix}
                &     & \ldots               \\
            x_i & y_i & 0      & 0   & 1 & 0 \\
            0   & 0   & x_i    & y_i & 0 & 1 \\
                &     & \ldots               \\
        \end{bmatrix}
        \begin{bmatrix}
            m_1 \\
            m_2 \\
            m_3 \\
            m_4 \\
            t_1 \\
            t_2 \\
        \end{bmatrix}
        =
        \begin{bmatrix}
            \ldots \\
            x'_i   \\
            y'_i   \\
            \ldots \\
        \end{bmatrix}
    \end{align*}
    And this is corresponding to the equation:
    $$\textbf{S}\textbf{h}=\textbf{u}$$
\end{proof}
c)\\
\textbf{Solution}\\
From b)
\begin{align}
    \textbf{h} = \textbf{S}^{-1} \textbf{u} \label{eq:1}
\end{align}
Transformation from the following points correspondences $\{(0,0)\rightarrow(1,2)\},
    \{(1,0)\rightarrow(3,2)\},\{(0,1)\rightarrow(1,4)\}$.
Equation\eqref{eq:1} becomes:
\begin{align*}
    \begin{bmatrix}
        m_1 \\
        m_2 \\
        m_3 \\
        m_4 \\
        t_1 \\
        t_2 \\
    \end{bmatrix}
     & =
    \begin{bmatrix}
        x_1 & y_1 & 0   & 0   & 1 & 0 \\
        0   & 0   & x_1 & y_1 & 0 & 1 \\
        x_2 & y_2 & 0   & 0   & 1 & 0 \\
        0   & 0   & x_2 & y_2 & 0 & 1 \\
        x_3 & y_3 & 0   & 0   & 1 & 0 \\
        0   & 0   & x_3 & y_3 & 0 & 1 \\
    \end{bmatrix}^{-1}
    \begin{bmatrix}
        x'_1 \\
        y'_1 \\
        x'_2 \\
        y'_2 \\
        x'_3 \\
        y'_3 \\
    \end{bmatrix} \\
     & =
    \begin{bmatrix}
        0 & 0 & 0 & 0 & 1 & 0 \\
        0 & 0 & 0 & 0 & 0 & 1 \\
        1 & 0 & 0 & 0 & 1 & 0 \\
        0 & 0 & 1 & 0 & 0 & 1 \\
        0 & 1 & 0 & 0 & 1 & 0 \\
        0 & 0 & 0 & 1 & 0 & 1 \\
    \end{bmatrix}^{-1}
    \begin{bmatrix}
        1 \\
        2 \\
        3 \\
        2 \\
        1 \\
        4 \\
    \end{bmatrix} \\
     & =
    \begin{bmatrix}
        2 \\
        0 \\
        0 \\
        2 \\
        1 \\
        2 \\
    \end{bmatrix} \\
\end{align*}
%\begin{align*}
%    \frac{\partial E}{\partial \textbf{M}} &= \frac{\partial}{\partial\textbf{M}}\sum_{i=1}^{n} ||\textbf{x}'_i-\textbf{M}\textbf{x}_i-\textbf{t}||^2\\
%    &= \frac{\partial}{\partial\textbf{M}}\sum_{i=1}^{n} (\textbf{x}'_i-\textbf{M}\textbf{x}_i-\textbf{t})^\top (\textbf{x}'_i-\textbf{M}\textbf{x}_i-\textbf{t})\\
%    &=\frac{\partial}{\partial\textbf{M}}\sum_{i=1}^{n} (\textbf{x}_i^{'\top}-\textbf{x}_i^{\top}\textbf{M}^{\top}-\textbf{t}^{\top}) (\textbf{x}'_i-\textbf{M}\textbf{x}_i-\textbf{t})\\
%    &=\sum_{i=1}^{n} \frac{\partial}{\partial\textbf{M}}(\textbf{x}_i^{'\top}-\textbf{x}_i^{\top}\textbf{M}^{\top}-\textbf{t}^{\top}) (\textbf{x}'_i-\textbf{M}\textbf{x}_i-\textbf{t})\\
%    &=\sum_{i=1}^{n} \frac{\partial}{\partial\textbf{M}}(\textbf{x}_i^{\top}\textbf{M}^{\top}\textbf{M}\textbf{x}_i-(\textbf{x}_i^{'\top}-\textbf{t}^\top)\textbf{M}\textbf{x}_i-\textbf{x}_i^{\top}\textbf{M}^{\top}(\textbf{x}'_i-\textbf{t}))\\
%    &=\sum_{i=1}^{n} 2(\textbf{x}_i^{\top}\textbf{M}^{\top}\textbf{x}_i-(\textbf{x}_i^{'\top}-\textbf{t}^\top)\textbf{x}_i)\\
%    &=2\sum_{i=1}^{n} (\textbf{x}_i^{\top}\textbf{M}^{\top}\textbf{x}_i-\textbf{x}_i^{'\top}\textbf{x}_i+\textbf{t}^\top\textbf{x}_i)\\
%\end{align*}
%\begin{align*}
%    \frac{\partial E}{\partial \textbf{t}} &= \frac{\partial}{\partial\textbf{t}}\sum_{i=1}^{n} ||\textbf{x}'_i-\textbf{M}\textbf{x}_i-\textbf{t}||^2\\
%    &=\frac{\partial}{\partial\textbf{t}}\sum_{i=1}^{n} (\textbf{x}'_i-\textbf{M}\textbf{x}_i-\textbf{t})^\top (\textbf{x}'_i-\textbf{M}\textbf{x}_i-\textbf{t})\\
%    &=\frac{\partial}{\partial\textbf{t}}\sum_{i=1}^{n} (\textbf{x}_i^{'\top}-\textbf{x}_i^{\top}\textbf{M}^{\top}-\textbf{t}^{\top}) (\textbf{x}'_i-\textbf{M}\textbf{x}_i-\textbf{t})\\
%    &=\sum_{i=1}^{n} \frac{\partial}{\partial\textbf{t}}(\textbf{x}_i^{'\top}-\textbf{x}_i^{\top}\textbf{M}^{\top}-\textbf{t}^{\top}) (\textbf{x}'_i-\textbf{M}\textbf{x}_i-\textbf{t})\\
%    &=\sum_{i=1}^{n} \frac{\partial}{\partial\textbf{t}}(\textbf{t}^\top\textbf{t}-(\textbf{x}_i^{'\top}-\textbf{x}_i^{\top}\textbf{M}^{\top})\textbf{t}-\textbf{t}^\top(\textbf{x}'_i-\textbf{M}\textbf{x}_i))\\
%    &=\sum_{i=1}^{n} (2\textbf{t}^\top-2(\textbf{x}_i^{'\top}-\textbf{x}_i^{\top}\textbf{M}^{\top}))\\
%    &=2\sum_{i=1}^{n} (\textbf{t}^\top-\textbf{x}_i^{'\top}+\textbf{x}_i^{\top}\textbf{M}^{\top})\\
%\end{align*}
\textbf{Exercise 2. Similarity transformation from two point correspondences.}\\
a)\\
\textbf{Solution}
\begin{align}
    \textbf{v}'                & = \textbf{x}'_2 - \textbf{x}'_1\nonumber                                \\
                               & = {s}\textbf{R}\textbf{x}_2 + \textbf{t} -
    {s}\textbf{R}\textbf{x}_1 - \textbf{t}\nonumber                                                      \\
                               & ={s}\textbf{R}(\textbf{x}_2-\textbf{x}_1)                               \\
    \nonumber                                                                                            \\
    \textbf{v}                 & = \textbf{x}_2 - \textbf{x}_1                                           \\
    \therefore \textbf{v}'     & = s\textbf{R}\textbf{v}                                                 \\
    \begin{bmatrix}
        v'_x \\
        v'_y
    \end{bmatrix}
                               & =
    s
    \begin{bmatrix}
        cos\theta & -sin\theta \\
        sin\theta & cos\theta
    \end{bmatrix}
    \begin{bmatrix}
        v_x \\
        v_y
    \end{bmatrix}\nonumber                                                                               \\
    v'_x                       & =s(cos\theta v_x - sin\theta v_y)\label{eq:5}                           \\
    v'_y                       & =s(sin\theta v_x + cos\theta v_y)    \label{eq:6}                       \\
    \intertext{From \eqref{eq:5}\eqref{eq:6}}\nonumber                                                   \\
    v'_x v_x + v'_y v_y        & = s(v_x^2+v_y^2)                                                        \\
    (v_x^{'2}+v_y^{'2})        & =s^2(v_x^2+v_y^2)                                                       \\
    \textbf{v}'\cdot\textbf{v} & = s |\textbf{v}|^2 cos\theta                                            \\
    |\textbf{v}'|              & =s|\textbf{v}|\label{eq:10}                                             \\
    \therefore cos\theta       & = \frac{\textbf{v}'\cdot\textbf{v}}{|\textbf{v}'||\textbf{v}|}\nonumber \\
    \theta                     & = arccos(\frac{\textbf{v}'\cdot\textbf{v}}{|\textbf{v}'||\textbf{v}|})
\end{align}

b)
\begin{proof}
    From \eqref{eq:10} above in a):
    \begin{align*}
        |\textbf{v}'| & =s|\textbf{v}|                       \\
        s             & = \frac{|\textbf{v}'|}{|\textbf{v}|}
    \end{align*}

\end{proof}

c)
\textbf{Solution}\\
\begin{align*}
    \textbf{t} & = \textbf{x}' - s\textbf{R}\textbf{x} \\
    \begin{bmatrix}
        t_x \\
        t_y
    \end{bmatrix}
               & =
    \begin{bmatrix}
        x' \\
        y'
    \end{bmatrix}
    -s
    \begin{bmatrix}
        cos\theta & -sin\theta \\
        sin\theta & cos\theta
    \end{bmatrix}
    \begin{bmatrix}
        x \\
        y
    \end{bmatrix}                                     \\
               & =
    \begin{bmatrix}
        x' - s(x cos\theta - y sin\theta) \\
        y' - s(x sin\theta + y cos\theta)
    \end{bmatrix}
\end{align*}

d)\\
\textbf{Solution}\\
Transformation from the following points correspondences $\{(1/2,0)\rightarrow(0,0)\},
    \{(0,1/2)\rightarrow(-1,-1)\}$.
\begin{align*}
    \textbf{v}'           & =
    \begin{bmatrix}
        -1 \\
        -1
    \end{bmatrix}                                                                                           \\
    \textbf{v}            & =
    \begin{bmatrix}
        -1/2 \\
        1/2
    \end{bmatrix}                                                                                           \\
    \theta                & = arccos(\frac{\textbf{v}'\cdot\textbf{v}}{|\textbf{v}'||\textbf{v}|})=arccos(0) \\
    \theta                & =\pi/2                                                                           \\
    \therefore \textbf{R} & =
    \begin{bmatrix}
        cos\theta & -sin\theta \\
        sin\theta & cos\theta
    \end{bmatrix}                                                                                   \\
                          & =
    \begin{bmatrix}
        0 & -1 \\
        1 & 0
    \end{bmatrix}                                                                                           \\
    \intertext{And}                                                                                          \\
    s                     & = \frac{|\textbf{v}'|}{|\textbf{v}|} = 2                                         \\
    \begin{bmatrix}
        t_x \\
        t_y
    \end{bmatrix}
                          & =
    \begin{bmatrix}
        x' - s(x cos\theta - y sin\theta) \\
        y' - s(x sin\theta + y cos\theta)
    \end{bmatrix}                                                                        \\
                          & =
    \begin{bmatrix}
        x' + sy \\
        y' - sx
    \end{bmatrix}                                                                                           \\
                          & =
    \begin{bmatrix}
        0 + 2 * 0 \\
        0 - 2 * 1/2
    \end{bmatrix}                                                                                           \\
                          & =
    \begin{bmatrix}
        0 \\
        -1
    \end{bmatrix}
\end{align*}

\end{document}
